\documentclass{article}
\usepackage{amsmath}
\begin{document}
\setlength{\parindent}{0in}

\textbf{fastbeta} for $S E I R$ equations:

\begin{subequations}
\begin{align}
  \frac{\text{d} E^{1}}{\text{d} t}
  &= \beta(t) S \sum\nolimits_{j} I^{j} - m \sigma E^{1} - \mu(t) E^{1} \\
  \frac{\text{d} E^{i}}{\text{d} t}
  &= m \sigma E^{i-1} - m \sigma E^{i} - \mu(t) E^{i} \\
  \frac{\text{d} I^{1}}{\text{d} t}
  &= m \sigma E^{m} - n \gamma I^{1} - \mu(t) I^{1} \\
  \frac{\text{d} I^{j}}{\text{d} t}
  &= n \gamma I^{j-1} - n \gamma I^{j} - \mu(t) I^{j} \\
  \frac{\text{d} R}{\text{d} t}
  &= n \gamma I^{n} - \delta R - \mu(t) R \\
  \frac{\text{d} S}{\text{d} t}
  &= \nu(t) + \delta R - \beta(t) S \sum\nolimits_{j} I^{j} - \mu(t) S
\end{align}
\end{subequations}

\begin{subequations}
\begin{align}
  E_{t+1}^{1} &= \frac{(1 - \frac{1}{2} (m \sigma + \mu_{t})) E_{t}^{1} + Z_{t+1}}{1 + \frac{1}{2} (m \sigma + \mu_{t+1})} \\
  E_{t+1}^{i} &= \frac{(1 - \frac{1}{2} (m \sigma + \mu_{t})) E_{t}^{i} + \frac{1}{2} m \sigma (E_{t}^{i-1} + E_{t+1}^{i-1})}{1 + \frac{1}{2} (m \sigma + \mu_{t+1})} \\
  I_{t+1}^{1} &= \frac{(1 - \frac{1}{2} (n \gamma + \mu_{t})) I_{t}^{1} + \frac{1}{2} m \sigma (E_{t}^{m} + E_{t+1}^{m})}{1 + \frac{1}{2} (n \gamma + \mu_{t+1})} \\
  I_{t+1}^{j} &= \frac{(1 - \frac{1}{2} (n \gamma + \mu_{t})) I_{t}^{j} + \frac{1}{2} n \gamma (I_{t}^{j-1} + I_{t+1}^{j-1})}{1 + \frac{1}{2} (n \gamma + \mu_{t+1})} \\
  R_{t+1} &= \frac{(1 - \frac{1}{2} (\delta + \mu_{t})) R_{t} + \frac{1}{2} n \gamma (I_{t}^{n} + I_{t+1}^{n})}{1 + \frac{1}{2} (\delta + \mu_{t+1})} \\
  S_{t+1} &= \frac{(1 - \frac{1}{2} \mu_{t}) S_{t} + B_{t+1} - Z_{t+1} + \frac{1}{2} \delta (R_{t} + R_{t+1})}{1 + \frac{1}{2} \mu_{t+1}} \\
  \beta_{t} &= \frac{Z_{t} + Z_{t+1}}{2 S_{t} \sum\nolimits_{j} I_{t}^{j}}
\end{align}
\end{subequations}

\end{document}
